proof/security/PKE_ROM.ec
@@ -1,4 +1,4 @@
-require import AllCore List Distr DBool PROM FinType.  
+require import AllCore List Distr DBool PROM FinType SmtMap.  
 require (****) LorR.
 
 abstract theory PKE.
@@ -138,14 +138,13 @@ qed.
 
 
 module OW_CPA (S:Scheme, A: OW_CPA_ADV) = {
+  var pk : pkey
+  var sk : skey
+  var m  : plaintext
+  var cc : ciphertext
+  var m' : plaintext option
 
   proc main_perfect() = {
-    var pk : pkey;
-    var m  : plaintext;
-    var m' : plaintext option;
-    var cc : ciphertext;
-    var sk : skey;
-
     (pk, sk) <@ S.kg();
     m        <$ dplaintext;
     cc       <@ S.enc(pk, m);
@@ -156,19 +155,14 @@ module OW_CPA (S:Scheme, A: OW_CPA_ADV) = {
 
   module O = {
     proc pco(sk, m : plaintext, c : ciphertext) : bool = {
-      var m';
-      m'   <@ S.dec(sk, c);
-      return m' = Some m;
+      var m'';
+      m''   <@ S.dec(sk, c);
+      return m'' = Some m;
     }
   }
 
   proc main() : bool = {
-    var pk : pkey;
-    var m  : plaintext;
-    var m' : plaintext option;
     var b  : bool;
-    var cc : ciphertext;
-    var sk : skey;
 
     (pk, sk) <@ S.kg();
     m        <$ dplaintext;
@@ -180,32 +174,29 @@ module OW_CPA (S:Scheme, A: OW_CPA_ADV) = {
 }.
 
 module BOWp(S : Scheme, A :  OW_CPA_ADV) : CORR_ADV = {
-   var m  : plaintext
-   var m' : plaintext option
    var m'' : plaintext option
-   var cc  : ciphertext
 
    proc find(pk : pkey, sk : skey) : plaintext = {
-       m  <$ dplaintext;
-    return m;
+       OW_CPA.m  <$ dplaintext;
+       return OW_CPA.m;
    }
 
    proc main() : bool = {
     var pk,sk;
     (pk, sk) <@ S.kg();
     find(pk,sk);
-    cc        <@ S.enc(pk, m);
-    m'        <@ A.find(pk,cc);
-    m''       <@ S.dec(sk, cc);
-    return (m'' <> Some m);
+    OW_CPA.cc <@ S.enc(pk, OW_CPA.m);
+    OW_CPA.m' <@ A.find(pk,OW_CPA.cc);
+    m''       <@ S.dec(sk, OW_CPA.cc);
+    return (m'' <> Some OW_CPA.m);
    }
 }.
 
 
 section.
 
-declare module S <: Scheme { -BOWp }.
-declare module A <: OW_CPA_ADV { -S, -BOWp }.
+declare module S <: Scheme { -BOWp, -OW_CPA }.
+declare module A <: OW_CPA_ADV { -S, -BOWp, -OW_CPA }.
 
 lemma ow_perfect &m : 
    islossless A.find =>
@@ -218,18 +209,18 @@ proof.
 move => A_ll Senc_ll Sdec_ll.
 have -> : 
   Pr[OW_CPA(S, A).main_perfect() @ &m : res] = 
-    Pr[ BOWp(S,A).main() @ &m : Some BOWp.m = BOWp.m' ].
+    Pr[ BOWp(S,A).main() @ &m : Some OW_CPA.m = OW_CPA.m' ].
 + byequiv => //.
   proc;inline *; seq 4 6 : #post; last by  conseq />;islossless.
-  conseq  (_: _ ==> m{1} = BOWp.m{2} /\ m'{1} = BOWp.m'{2}); 1: by smt().
+  conseq  (_: _ ==> OW_CPA.m{1} = OW_CPA.m{2} /\ OW_CPA.m'{1} = OW_CPA.m'{2}); 1: by smt().
   by sim.
 
 have -> : 
   Pr[OW_CPA(S, A).main() @ &m : res] = 
-    Pr[ BOWp(S,A).main() @ &m : if BOWp.m' = None then false else BOWp.m'' = BOWp.m'].
+    Pr[ BOWp(S,A).main() @ &m : if OW_CPA.m' = None then false else BOWp.m'' = OW_CPA.m'].
 + byequiv => //.
   proc;inline *; seq 9 7 : #post; last by conseq />; islossless. 
-  wp. conseq (: m'{1} = BOWp.m'{2} /\ m'0{1} = BOWp.m''{2} /\ m0{1} = oget BOWp.m'{2}); 1: smt().
+  wp. conseq (: OW_CPA.m'{1} = OW_CPA.m'{2} /\ m''{1} = BOWp.m''{2} /\ m{1} = oget OW_CPA.m'{2}); 1: smt().
   by call(:true);wp;call(:true);wp;call(:true);rnd;wp;call(:true);auto.
 
 have -> : 
@@ -237,7 +228,7 @@ have -> :
     Pr[ BOWp(S,A).main() @ &m : res ].
 + byequiv => //.
   proc;inline *. swap {2} 6 1. call{2}(:true ==> true). 
-  wp; conseq (: m'{1} = BOWp.m''{2} /\ m{1} = BOWp.m{2} ); 1: smt().
+  wp; conseq (: m'{1} = BOWp.m''{2} /\ m{1} = OW_CPA.m{2} ); 1: smt().
   by sim.
 
 byequiv : (res) => //.
@@ -248,6 +239,8 @@ qed.
 end section.
 
 (* Ind implies ow for large message spaces *)
+
+theory OWvsIND.
 
 module Bow(A :  OW_CPA_ADV) : Adversary = {
    var m0, m1  : plaintext
@@ -276,8 +269,8 @@ module Bow(A :  OW_CPA_ADV) : Adversary = {
 section.
 
 
-declare module S <: Scheme {-Bow, -BOWp}.
-declare module A <: OW_CPA_ADV {-S, -Bow, -BOWp}.
+declare module S <: Scheme {-Bow, -BOWp, -OW_CPA}.
+declare module A <: OW_CPA_ADV {-S, -Bow, -BOWp, -OW_CPA}.
 
 local module Aux = {
   proc main0() : bool = {
@@ -404,6 +397,228 @@ have -> : Pr[CPA_R(S, Bow(A)).main() @ &m : res /\ ! (Bow.m = None \/ (Bow.m <> 
 qed.
 
 end section.
+
+end OWvsIND.
+
+(* Ind tightly implies even list OW for large message spaces *)
+
+theory OWvsIND_RO.
+
+clone import FullRO as RO with
+   type in_t <- plaintext
+   proof *.
+
+(* 
+module O_AdvOW = {
+  var pk : pkey
+  proc pco(m : plaintext, c : ciphertext) : bool = {
+    var r, c';
+    r  <@ RO.RO.get(m);
+    c' <- enc r pk m;
+    return c = c';
+  }
+  
+  proc cvo(c:ciphertext) : bool = {
+    var rv; 
+    rv <- false; 
+    if (c <> OW_PCVA.cc) 
+      rv <- find (fun m r => c = enc r pk m) RO.RO.m <> None;
+    return rv;
+  }
+}.
+
+module AdvOW_query (A:PCVA_ADV) = {
+  import var OW_PCVA O_AdvOW
+
+  module A = A(CountH(RO.RO), CountO(O_AdvOW))
+
+  proc main(pk0:pkey, c:ciphertext) : unit = {
+    var m' : plaintext option;
+    pk <- pk0; 
+    RO.RO.init();
+    cc       <- c; 
+    CountO(O_AdvOW).init();
+    m'       <@ A.find(pk,cc);
+  }
+
+  proc find(pk0:pkey, c:ciphertext) : plaintext option = {
+    var i : int;
+    main(pk0, c);
+    i        <$ [0 .. qH + qP - 1];
+    return Some (nth witness (elems (fdom RO.RO.m)) i);
+  }
+}.
+*)
+
+module BowROM(A :  OW_CPA_ADV) : Adversary = {
+   var m0, m1  : plaintext
+   var pk      : pkey
+
+   proc choose(_pk : pkey) : plaintext * plaintext = {
+     pk <- _pk;
+     RO.init();
+     m0 <$ dplaintext;
+     m1 <$ dplaintext;
+     return (m0,m1);
+   }
+
+   proc guess(c : ciphertext) : bool = {
+      var b;
+      b <$ {0,1};
+      A.find(pk,c);
+      return if (m0 \in RO.m = m1 \in RO.m)
+             then b
+             else if (m0 \in RO.m) 
+                  then false 
+                  else true;
+   }
+}.
+
+section.
+
+
+declare module S <: Scheme {-BowROM, -BOWp, -OW_CPA}.
+declare module A <: OW_CPA_ADV {-S,  -BOWp, -OW_CPA}.
+
+local module Aux = {
+  proc main0() : bool = {
+   var pk,sk,c,b;
+   (pk, sk) <@ S.kg();                                                
+   BowROM.pk <- pk;                                                       
+   BowROM.m0 <$ dplaintext;                                                
+   BowROM.m1 <$ dplaintext;                                               
+   c <@ S.enc(pk, BowROM.m0);                                                
+   b <$ {0,1};                                                        
+   A.find(pk,c);
+   return if (BowROM.m0 \in RO.m = BowROM.m1 \in RO.m)
+          then b
+          else if (BowROM.m0 \in RO.m) 
+               then false 
+               else true;
+  }
+
+  proc main1() : bool = {
+   var pk,sk,c,b;
+   (pk, sk) <@ S.kg();                                                
+   BowROM.pk <- pk;                                                       
+   BowROM.m0 <$ dplaintext;                                                
+   BowROM.m1 <$ dplaintext;                                               
+   c <@ S.enc(pk, BowROM.m1);                                                
+   b <$ {0,1};                                                        
+   A.find(pk,c);
+   return if (BowROM.m0 \in RO.m = BowROM.m1 \in RO.m)
+          then b
+          else if (BowROM.m0 \in RO.m) 
+               then false 
+               else true;
+  }
+
+}.
+
+lemma ow_ind_ro &m : 
+   islossless S.kg =>
+   islossless S.enc =>
+   islossless S.dec =>
+   islossless A.find =>
+
+   Pr[ OW_CPA(S,A).main() @ &m :   OW_CPA.m \in RO.m] <=
+      2%r * (eps_msg + 
+        `| Pr[CPA(S,BowROM(A)).main() @ &m : res] - 1%r/2%r |) + 
+             Pr[ Correctness_Adv(S,BOWp(S,A)).main() @ &m : res ].   
+admitted. 
+(* 
+proof. 
+move => kg_ll enc_ll dec_ll A_ll. 
+have : Pr[ OW_CPA(S,A).main_perfect() @ &m : res ] <=
+      2%r * (eps_msg + 
+        `| Pr[CPA(S,Bow(A)).main() @ &m : res] - 1%r/2%r |); last 
+ by move : (ow_perfect  S A &m A_ll enc_ll dec_ll);smt().
+
+rewrite RField.mulrDr -(pr_CPA_LR S (Bow(A)) &m kg_ll enc_ll); 1,2: by islossless.
+have -> : 
+  Pr[CPA_L(S, Bow(A)).main() @ &m : res] = 
+  Pr[CPA_L(S, Bow(A)).main() @ &m : res /\ (Bow.m = None \/ (Bow.m <> Some Bow.m0 /\ Bow.m <> Some Bow.m1))] + 
+  Pr[CPA_L(S, Bow(A)).main() @ &m : res /\ !(Bow.m = None \/ (Bow.m <> Some Bow.m0 /\ Bow.m <> Some Bow.m1))]
+by rewrite Pr[mu_split (Bow.m = None \/ (Bow.m <> Some Bow.m0 /\ Bow.m <> Some Bow.m1))] => /#.
+
+have -> : 
+  Pr[CPA_R(S, Bow(A)).main() @ &m : res] = 
+  Pr[CPA_R(S, Bow(A)).main() @ &m : res /\ (Bow.m = None \/ (Bow.m <> Some Bow.m0 /\ Bow.m <> Some Bow.m1))] + 
+  Pr[CPA_R(S, Bow(A)).main() @ &m : res /\ !(Bow.m = None \/ (Bow.m <> Some Bow.m0 /\ Bow.m <> Some Bow.m1))]
+by rewrite Pr[mu_split (Bow.m = None \/ (Bow.m <> Some Bow.m0 /\ Bow.m <> Some Bow.m1))] => /#.
+
+have ->  /=: 
+  Pr[CPA_L(S, Bow(A)).main() @ &m : res /\ (Bow.m = None \/ (Bow.m <> Some Bow.m0 /\ Bow.m <> Some Bow.m1))] =
+  Pr[CPA_R(S, Bow(A)).main() @ &m : res /\ (Bow.m = None \/ (Bow.m <> Some Bow.m0 /\ Bow.m <> Some Bow.m1))].
++ byequiv (: _ ==> (res /\ (Bow.m = None \/ (Bow.m <> Some Bow.m0 /\ Bow.m <> Some Bow.m1))){1} <=>
+                   (res /\ (Bow.m = None \/ (Bow.m <> Some Bow.m0 /\ Bow.m <> Some Bow.m1))){2}) => //.
+  proc. 
+  seq 2 2 : (={glob A, glob S, pk,sk, Bow.pk} /\ 
+             Bow.m0{1} = Bow.m1{2} /\ Bow.m1{1} = Bow.m0{2} /\ Bow.pk{1} = pk{1} /\
+             Bow.m0{1} = m0{1} /\ Bow.m1{1} = m1{1} /\
+             Bow.m0{2} = m0{2} /\ Bow.m1{2} = m1{2});
+     1: by inline *;swap {1} 4 1;auto;call(_: true); auto.
+  by inline *;wp;call(_: true);rnd;wp;call(_:true);auto => /> /#.
+
+have : 
+   Pr[CPA_L(S, Bow(A)).main() @ &m : res /\ ! (Bow.m = None \/ (Bow.m <> Some Bow.m0 /\ Bow.m <> Some Bow.m1))] <= eps_msg.
++ have -> : Pr[CPA_L(S, Bow(A)).main() @ &m : res /\ ! (Bow.m = None \/ (Bow.m <> Some Bow.m0 /\ Bow.m <> Some Bow.m1))] = 
+            Pr[Aux.main0() @ &m : res /\ ! (Bow.m = None \/ (Bow.m <> Some Bow.m0 /\ Bow.m <> Some Bow.m1))]
+   by byequiv => //;proc;inline *;wp;conseq />; sim. 
+  byphoare => //. 
+  proc;inline *; swap 4 3.
+  conseq (: _ ==> Some Bow.m1 = Bow.m); 1: by smt().
+  seq 6 : true  (1%r)  (eps_msg) (0%r) (0%r).
+  + by trivial.
+  + by trivial. 
+  + rnd; skip => /> &hr.  
+    case(Bow.m{hr} = None); 1: by move => -> /=; rewrite mu0;smt(MFinT.card_gt0).
+    move => nnone.
+    have -> : (fun (x : plaintext) => Some x = Bow.m{hr})  = pred1 (oget Bow.m{hr}) by apply fun_ext => x;smt().
+    by smt(eps_msgE).
+     + by hoare; trivial.
+  by trivial.
+  
+have : 
+  `| Pr[OW_CPA(S, A).main_perfect() @ &m : res] - 
+      Pr[CPA_R(S, Bow(A)).main() @ &m : res /\ ! (Bow.m = None \/ (Bow.m <> Some Bow.m0 /\ Bow.m <> Some Bow.m1))]| <= 
+         eps_msg; last by smt().
+
+have -> : Pr[OW_CPA(S, A).main_perfect() @ &m : res] = 
+            Pr[Aux.main1()           @ &m : Bow.m = Some Bow.m1]
+     by byequiv => //;proc;inline*;wp;call(_: true);rnd{2};
+        call(:true);rnd;rnd{2};wp;call(_: true);auto => />.
+
+have -> : Pr[CPA_R(S, Bow(A)).main() @ &m : res /\ ! (Bow.m = None \/ (Bow.m <> Some Bow.m0 /\ Bow.m <> Some Bow.m1))] = 
+            Pr[Aux.main1()           @ &m : res /\ ! (Bow.m = None \/ (Bow.m <> Some Bow.m0 /\ Bow.m <> Some Bow.m1))]
+      by byequiv => //;proc;inline*;wp;conseq />;sim.
+
+  have  : Pr[Aux.main1() @ &m : !res /\  !(Bow.m <> Some Bow.m0 /\ Bow.m <> Some Bow.m1)] <= 
+            eps_msg.
+  + byphoare => //. 
+    proc;inline *;swap 3 4.
+    conseq (: _ ==> Bow.m0 = oget Bow.m); 1: by smt().
+    seq 6 : true  (1%r)  (eps_msg) (0%r) (0%r).
+    + by trivial.
+    + by islossless. 
+    + rnd; skip => />*; rewrite eps_msgE /#.
+    + by hoare; trivial. 
+    by trivial. 
+
+  have : `|Pr[Aux.main1() @ &m : Bow.m = Some Bow.m1] -
+  Pr[Aux.main1() @ &m : res /\ ! (Bow.m = None \/ Bow.m <> Some Bow.m0 /\ Bow.m <> Some Bow.m1)]|  <=
+      Pr[Aux.main1() @ &m : !res /\ ! (Bow.m <> Some Bow.m0 /\ Bow.m <> Some Bow.m1)]; last by smt().
+  byequiv : (!res /\ ! (Bow.m = None \/ (Bow.m <> Some Bow.m0 /\ Bow.m <> Some Bow.m1))) => //. 
+  + proc;inline *.
+    by call(:true);rnd;call(:true);rnd;rnd;wp;call(:true);auto => /> /#.
+    
+qed.
+*)
+
+end section.
+
+end OWvsIND_RO.
+
 
 end PKE.
 
@@ -653,3 +868,4 @@ module OW_PCVA (H : Oracle, S:Scheme, A: PCVA_ADV) = {
 }.
 
 end PKE_ROM.
+
